Definition of sublist. Removed dependency on Imperative_HOL/ex/Subarray.

HOL/DataStrs/Reverse_Func.thy
@@ -108,20 +108,26 @@ lemma rev_swap_eval [rewrite]:
 lemma rev_swap_is_rev [rewrite]:
   "length xs \<ge> 1 \<Longrightarrow> rev_swap xs 0 (length xs - 1) = rev xs" by auto2
 
-section {* take and drop *}
+section {* take *}
 
 setup {* register_wellform_data ("take n xs", ["n \<le> length xs"]) *}
 setup {* add_prfstep_check_req ("take n xs", "n \<le> length xs") *}
-lemma length_take': "n \<le> length xs \<Longrightarrow> length (take n xs) = n" by simp
-setup {* add_rewrite_rule_cond @{thm length_take'} [with_term "take ?n ?xs"] *}
-lemma nth_take' [rewrite]: "i < length (take n xs) \<Longrightarrow> take n xs ! i = xs ! i" by simp
+
+lemma length_take: "n \<le> length xs \<Longrightarrow> length (take n xs) = n" by simp
+setup {* add_rewrite_rule_cond @{thm length_take} [with_term "take ?n ?xs"] *}
+
+lemma nth_take [rewrite]: "i < length (take n xs) \<Longrightarrow> take n xs ! i = xs ! i" by simp
+
 setup {* add_rewrite_rule @{thm List.take_0} *}
 
-setup {* add_rewrite_rule_cond @{thm List.length_drop} [with_term "drop ?n ?xs"] *}
-lemma nth_drop' [rewrite]: "i < length (drop n xs) \<Longrightarrow> drop n xs ! i = xs ! (n + i)" by simp
-setup {* add_rewrite_rule @{thm List.drop_0} *}
+section {* drop *}
 
-setup {* add_rewrite_rule @{thm List.append_take_drop_id} *}
+setup {* add_rewrite_rule_cond @{thm List.length_drop} [with_term "drop ?n ?xs"] *}
+
+lemma nth_drop [rewrite]: "i < length (drop n xs) \<Longrightarrow> drop n xs ! i = xs ! (n + i)" by simp
+
+setup {* add_rewrite_rule @{thm List.drop_0} *}
+setup {* add_rewrite_rule @{thm List.drop_all} *}
 
 section {* Copy one array to the beginning of another *}
     
@@ -157,8 +163,96 @@ setup {* del_prfstep_thm @{thm array_copy.simps} *}
 lemma array_copy_take [backward]:
   "n \<le> length xs' \<Longrightarrow> n \<le> length xs \<Longrightarrow> take n (array_copy xs 0 xs' 0 n) = take n xs"
 @proof
-  @have "length (array_copy xs 0 xs' 0 n) = length xs'"
   @have "length (take n (array_copy xs 0 xs' 0 n)) = length (take n xs)"
 @qed
+
+section {* Sublist *}
+
+definition sublist :: "nat \<Rightarrow> nat \<Rightarrow> 'a list \<Rightarrow> 'a list" where [rewrite]:
+  "sublist l r xs = drop l (take r xs)"
+setup {* register_wellform_data ("sublist l r xs", ["l \<le> r", "r \<le> length xs"]) *}
+setup {* add_prfstep_check_req ("sublist l r xs", "l \<le> r \<and> r \<le> length xs") *}
+
+lemma length_sublist:
+  "r \<le> length xs \<Longrightarrow> length (sublist l r xs) = r - l" by auto2
+setup {* add_forward_prfstep_cond @{thm length_sublist} [with_term "sublist ?l ?r ?xs"] *}
+
+lemma nth_sublist [rewrite]:
+  "r \<le> length xs \<Longrightarrow> xs' = sublist l r xs \<Longrightarrow> i < length xs' \<Longrightarrow> xs' ! i = xs ! (i + l)" by auto2
+
+lemma sublist_nil [rewrite]:
+  "r \<le> length xs \<Longrightarrow> r \<le> l \<Longrightarrow> sublist l r xs = []" by auto2
+
+setup {* del_prfstep_thm @{thm sublist_def} *}
+
+lemma sublist_single [rewrite]:
+  "l + 1 \<le> length xs \<Longrightarrow> sublist l (l + 1) xs = [xs ! l]"
+@proof @have "length [xs ! l] = 1" @qed
+
+lemma nat_sub7 [rewrite]: "b \<le> a \<Longrightarrow> c \<le> b \<Longrightarrow> ((a::nat) - b) + (b - c) = a - c" by simp
+lemma nat_sub8 [rewrite]: "b \<ge> c \<Longrightarrow> a \<ge> b - c \<Longrightarrow> (a::nat) - (b - c) + b = a + c" by simp
+
+lemma sublist_as_append [rewrite]:
+  "l \<le> m \<Longrightarrow> m \<le> r \<Longrightarrow> r \<le> length xs \<Longrightarrow> sublist l m xs @ sublist m r xs = sublist l r xs"
+@proof
+  @let "xs1 = sublist l r xs" "xs2 = sublist l m xs" "xs3 = sublist m r xs"
+  @have "length (xs2 @ xs3) = (r - m) + (m - l)"
+  @have "\<forall>i<length xs1. xs1 ! i = (xs2 @ xs3) ! i" @with
+    @case "i < length xs2" @then
+    @have "i - length xs2 < length xs3"
+  @end
+@qed
+
+lemma sublist_as_Cons [rewrite]:
+  "r \<le> length xs \<Longrightarrow> l < r \<Longrightarrow> xs ! l # sublist (l + 1) r xs = sublist l r xs"
+@proof
+  @have "sublist l r xs = sublist l (l + 1) xs @ sublist (l + 1) r xs"
+@qed
+
+lemma sorted_triv_list [backward]:
+  "r + 1 \<le> length xs \<Longrightarrow> l \<ge> r \<Longrightarrow> sorted (sublist l (r + 1) xs)"
+@proof @case "l = r" @qed
+
+setup {* add_rewrite_rule @{thm sorted_append} *}
+lemma sorted_pivoted_list [forward]:
+  "l \<le> p \<Longrightarrow> p + 1 \<le> r \<Longrightarrow> r \<le> length xs \<Longrightarrow>
+   sorted (sublist (p + 1) r xs) \<Longrightarrow> sorted (sublist l p xs) \<Longrightarrow>
+   \<forall>x\<in>set (sublist l p xs). x \<le> xs ! p \<Longrightarrow> \<forall>y\<in>set (sublist (p + 1) r xs). xs ! p \<le> y \<Longrightarrow>
+   sorted (sublist l r xs)"
+@proof
+  @have "sublist p r xs = (xs ! p) # sublist (p + 1) r xs" @then
+  @case "p = 0"
+  @have "sublist l r xs = sublist l p xs @ sublist p r xs"
+@qed
+setup {* del_prfstep_thm @{thm sorted_append} *}
+
+lemma sublist_equalityI:
+  "i \<le> j \<Longrightarrow> j \<le> length xs \<Longrightarrow> length xs = length ys \<Longrightarrow>
+   \<forall>k. i \<le> k \<longrightarrow> k < j \<longrightarrow> xs ! k = ys ! k \<Longrightarrow> sublist i j xs = sublist i j ys"
+@proof
+  @let "xs1 = sublist i j xs" "xs2 = sublist i j ys"
+  @have "\<forall>k<j-i. xs1 ! k = xs2 ! k" @with @have "i \<le> i + k" @end
+@qed
+setup {* add_backward2_prfstep_cond @{thm sublist_equalityI} [with_filt (order_filter "xs" "ys")] *}
+
+lemma set_sublist [resolve]:
+  "j \<le> length xs \<Longrightarrow> x \<in> set (sublist i j xs) \<Longrightarrow> \<exists>k. k \<ge> i \<and> k < j \<and> x = xs ! k"
+@proof
+  @let "xs' = sublist i j xs" @have "length xs' = j - i"
+  @obtain l where "l < length xs'" "x = xs' ! l"
+  @have "x = xs ! (l + i)"
+  @have "i + l \<ge> i"
+@qed
+
+lemma list_take_sublist_drop_eq [rewrite]:
+  "l \<le> r \<Longrightarrow> r \<le> length xs \<Longrightarrow> take l xs @ sublist l r xs @ drop r xs = xs"
+@proof
+  @have "take l xs = sublist 0 l xs" @with @have "length (take l xs) = l" @end
+  @have "drop r xs = sublist r (length xs) xs" @with @have "length (drop r xs) = length xs - r" @end
+@qed
+
+setup {* add_rewrite_rule @{thm mset_append} *}
+setup {* add_forward_prfstep @{thm add_right_imp_eq} *}
+setup {* add_forward_prfstep @{thm add_left_imp_eq} *}
 
 end
