HOL/SepLogic/More_Lists.thy
@@ -1,5 +1,5 @@
 theory More_Lists
-imports "../DataStrs/Lists_Ex" "~~/src/HOL/Imperative_HOL/ex/Subarray"
+imports "../DataStrs/Lists_Ex"
 begin
 
 section {* More on take, drop, and update *}
@@ -42,9 +42,6 @@ section {* Relationship between mset and set of lists *}
 setup {* add_rewrite_rule_cond @{thm in_multiset_in_set} [with_term "set ?xs"] *}
 setup {* add_rewrite_rule_back_cond @{thm in_multiset_in_set} [with_term "mset ?xs"] *}
 
-theorem in_set_conv_nth' [resolve]: "x \<in> set xs \<Longrightarrow> \<exists>i<length xs. x = xs ! i"
-  by (metis in_set_conv_nth)
-
 theorem in_mset_conv_nth [resolve]: "x \<in># mset xs \<Longrightarrow> \<exists>i<length xs. x = xs ! i"
   by (simp add: in_set_conv_nth')
 
@@ -58,51 +55,5 @@ theorem delete_mset_to_set [rewrite]:
 theorem update_mset_to_set [rewrite]:
   "mset xs' = {# y #} + (mset xs - {# x #}) \<Longrightarrow> distinct xs \<Longrightarrow> set xs' = (set xs - {x}) \<union> {y}"
   by (metis insert_mset_to_set mset_remove1 set_remove1_eq union_commute)
-
-section {* Sublist *}
-
-setup {* add_backward2_prfstep (equiv_backward_th @{thm sublist'_eq_samelength_iff}) *}
-setup {* add_rewrite_rule @{thm length_sublist'} *}
-
-theorem sublist_as_Cons [backward]:
-  "l < r \<Longrightarrow> r \<le> length xs \<Longrightarrow> sublist' l r xs = xs ! l # sublist' (l + 1) r xs"
-  by (metis One_nat_def add.right_neutral add_Suc_right order_less_trans sublist'_front le_neq_implies_less)
-theorem sublist_as_append [backward]:
-  "l \<le> m \<Longrightarrow> m \<le> r \<Longrightarrow> sublist' l r xs = sublist' l m xs @ sublist' m r xs"
-  by (simp add: sublist'_append)
-
-(* An result about sortedness of trivial sublists. *)
-theorem sublist'_single' [rewrite]:
-  "n < length xs \<Longrightarrow> sublist' n (n + 1) xs = [xs ! n]" using sublist'_single by simp
-setup {* fold add_rewrite_rule [@{thm sublist'_Nil'}, @{thm sublist'_Nil2}] *}
-
-(* Some results about sets and multisets of sublists. *)
-setup {* add_rewrite_rule @{thm set_sublist'} *}
-lemma set_sublistD [forward]:
-  "x \<in> set (sublist' i j xs) \<Longrightarrow> \<exists>k. k \<ge> i \<and> k < j \<and> k < length xs \<and> x = xs ! k" by auto2
-setup {* del_prfstep_thm @{thm set_sublist'} *}
-
-theorem mset_sublist' [backward1]:
-  "r \<le> List.length xs \<Longrightarrow> \<forall>i. i < l \<longrightarrow> xs ! i = ys ! i \<Longrightarrow> \<forall>i. i \<ge> r \<longrightarrow> xs ! i = ys ! i \<Longrightarrow>
-   mset xs = mset ys \<Longrightarrow> mset (sublist' l r xs) = mset (sublist' l r ys)"
-  by (smt le_less_trans mset_eq_length mset_sublist nat_less_le sublist'_eq_samelength_iff)
-
-(* Sortedness of lists of form x @ [pivot] @ y. *)
-setup {* add_rewrite_rule @{thm sorted_append} *}
-lemma sorted_pivoted_list [forward]: "sorted (sublist' (p + 1) r xs) \<Longrightarrow> sorted (sublist' l p xs) \<Longrightarrow>
-  \<forall>x\<in>set (sublist' l p xs). x \<le> xs ! p \<Longrightarrow> \<forall>y\<in>set (sublist' (p + 1) r xs). xs ! p \<le> y \<Longrightarrow>
-  l \<le> p \<Longrightarrow> p < r \<Longrightarrow> r \<le> length xs \<Longrightarrow> sorted (sublist' l r xs)"
-@proof
-  @have "sublist' p r xs = xs ! p # sublist' (p + 1) r xs" @then
-  @case "p = 0" @then
-  @have "sublist' l r xs = sublist' l p xs @ sublist' p r xs"
-@qed
-setup {* del_prfstep_thm @{thm sorted_append} *}
-
-lemma sorted_triv_list: "l \<ge> r \<Longrightarrow> sorted (sublist' l (r + 1) xs)"
-@proof
-  @case "l \<ge> length xs" @then @case "l = r" @then @have "l > r"
-@qed
-setup {* add_forward_prfstep_cond @{thm sorted_triv_list} [with_term "sublist' ?l (?r + 1) ?xs"] *}
 
 end
